Flapjack/Test/RiscVMemory.lean
@@ -41,6 +41,21 @@ example :
   native_decide
 
 example :
+    panRiscVRead16 riscvFlatTestDomain riscvFlatTestMemory
+      (BitVec.ofNat 64 8) (BitVec.ofNat 64 8) =
+      some (BitVec.ofNat 64 513) := by
+  native_decide
+
+example :
+    (do
+      let memory ← panRiscVStore16 riscvFlatTestDomain riscvFlatZeroMemory
+        (BitVec.ofNat 64 8) (BitVec.ofNat 64 8) (BitVec.ofNat 64 48879)
+      panRiscVRead16 riscvFlatTestDomain memory
+        (BitVec.ofNat 64 8) (BitVec.ofNat 64 8)) =
+      some (BitVec.ofNat 64 48879) := by
+  native_decide
+
+example :
     evalPanRiscVFlatResult [] (BitVec.ofNat 64 0) (BitVec.ofNat 64 100)
       (BitVec.ofNat 64 8) (fun _ => none) (fun _ => none)
       riscvFlatTestDomain riscvFlatZeroMemory
@@ -61,10 +76,39 @@ example :
       (.seq (.storeByte (.const (BitVec.ofNat 64 9))
           (.const (BitVec.ofNat 64 7)))
         (.return (.loadByte (.const (BitVec.ofNat 64 9))))) =
-      some [.word (BitVec.ofNat 64 7)] := by
+    some [.word (BitVec.ofNat 64 7)] := by
   simp [evalPanRiscVFlatResult, evalPanRiscVFlatProg, evalPanRiscVFlatExp,
     panRiscVStoreByte, panRiscVReadByte, panRiscVGetByte, panRiscVSetByte,
     panRiscVByteAlign, panRiscVByteIndex, riscvFlatTestDomain,
+    riscvFlatZeroMemory, updatePanValueMap, byteAddress, aligned]
+
+example :
+    evalPanRiscVFlatResult [] (BitVec.ofNat 64 0) (BitVec.ofNat 64 100)
+      (BitVec.ofNat 64 8) (fun _ => none) (fun _ => none)
+      riscvFlatTestDomain riscvFlatTestMemory
+      (.seq (.shMemLoad .op16 .local "x" (.const (BitVec.ofNat 64 8)))
+        (.return (.var .local "x"))) =
+      some [.word (BitVec.ofNat 64 513)] := by
+  simp [evalPanRiscVFlatResult, evalPanRiscVFlatProg,
+    evalPanRiscVFlatExp, panRiscVReadShared, panRiscVRead16,
+    panRiscVReadByte, panRiscVGetByte, panRiscVByteAlign,
+    panRiscVByteIndex, riscvFlatTestDomain, riscvFlatTestMemory,
+    updatePanValueMap, byteAddress, aligned]
+
+example :
+    evalPanRiscVFlatResult [] (BitVec.ofNat 64 0) (BitVec.ofNat 64 100)
+      (BitVec.ofNat 64 8) (fun _ => none) (fun _ => none)
+      riscvFlatTestDomain riscvFlatZeroMemory
+      (.seq (.shMemStore .op16 (.const (BitVec.ofNat 64 8))
+          (.const (BitVec.ofNat 64 48879)))
+        (.seq (.shMemLoad .op16 .local "x" (.const (BitVec.ofNat 64 8)))
+          (.return (.var .local "x")))) =
+      some [.word (BitVec.ofNat 64 48879)] := by
+  simp [evalPanRiscVFlatResult, evalPanRiscVFlatProg,
+    evalPanRiscVFlatExp, panRiscVReadShared, panRiscVRead16,
+    panRiscVReadByte, panRiscVGetByte, panRiscVByteAlign,
+    panRiscVByteIndex, panRiscVStoreShared, panRiscVStore16,
+    panRiscVStoreByte, panRiscVSetByte, riscvFlatTestDomain,
     riscvFlatZeroMemory, updatePanValueMap, byteAddress, aligned]
 
 end Flapjack
